P1.fst
@@ -13,15 +13,104 @@ module U = FStar.UInt64
 
 open NTreeC3
 
-inline_for_extraction noextract
-let one = U.uint_to_t 1
-inline_for_extraction noextract
-let zero = U.uint_to_t 0
 
 /// The implementation of the Selectors.Tree interface.
 /// Predicates prefixed by (**) correspond to stateful lemmas for folding and unfolding the tree predicate
 
 #set-options "--fuel 1 --ifuel 1 --z3rlimit 50 --ide_id_info_off"
+
+let create_leaf (#a: Type0) (_: unit) : Steel (t a)
+  emp (fun ptr -> linked_tree ptr)
+  (requires fun _ -> True)
+  (ensures fun _ ptr h1 ->
+    v_linked_tree ptr h1 == Trees.Leaf)
+  = intro_linked_tree_leaf ();
+    // TODO: it should be possible to remove next line
+    let h = get () in
+    return null_t
+
+let create_tree (#a: Type0) (v: a) : Steel (t a)
+  emp (fun ptr -> linked_tree ptr)
+  (requires fun _ -> True)
+  (ensures fun _ ptr h1 ->
+    v_linked_tree ptr h1 ==
+    Trees.Node v Trees.Leaf Trees.Leaf (U.v one))
+  =
+  let l = create_leaf () in
+  let r = create_leaf () in
+  let sr = malloc 1UL in
+  let n = mk_node v l r sr in
+  let ptr = malloc n in
+  NTreeC3.pack_tree ptr l r sr;
+  return ptr
+
+let sot_wds (#a: Type) (ptr: t a)
+  : Steel (U.t)
+  (linked_tree ptr)
+  (fun _ -> linked_tree ptr)
+  (requires fun _ -> True)
+  (ensures (fun h0 s h1 ->
+    v_linked_tree ptr h0 == v_linked_tree ptr h1 /\
+    U.v s == Spec.sot_wds (v_linked_tree ptr h0) /\
+    U.v s == Spec.size_of_tree (v_linked_tree ptr h0)
+  ))
+  =
+  if is_null_t ptr then (
+    assert (is_null_t ptr);
+    elim_linked_tree_leaf ptr;
+    let h = get () in
+    assert (0 == Spec.sot_wds (v_linked_tree ptr h));
+    return zero
+  ) else (
+    let h1 = get () in
+    (**) let node = unpack_tree ptr in
+    let h2 = get () in
+    let ptr_t1 = hide (v_linked_tree ptr h1) in
+    let ptr_t2 = hide (Spec.Node
+      (get_data (sel ptr h2))
+      (v_linked_tree (get_left node) h2)
+      (v_linked_tree (get_right node) h2)
+      (U.v (sel (get_size node) h2))
+    ) in
+    assert (reveal ptr_t1 == reveal ptr_t2);
+    assert (fst (Spec.is_wds (reveal ptr_t1)));
+    let ptr_s1 = hide (Spec.csize ptr_t1) in
+    let ptr_s2 = hide (Spec.csize ptr_t2) in
+    assert (reveal ptr_s1 == reveal ptr_s2);
+    Spec.check (reveal ptr_t1);
+    assert (reveal ptr_s1 == Spec.size_of_tree (reveal ptr_t1));
+    let s = read (get_size node) in
+    assert (U.v s == Spec.sot_wds (v_linked_tree ptr h1));
+    pack_tree ptr (get_left node) (get_right node) (get_size node);
+    return s
+  )
+
+let merge_tree (#a: Type0) (v: a) (l: t a) (r: t a) : Steel (t a)
+  (linked_tree l `star` linked_tree r)
+  (fun ptr -> linked_tree ptr)
+  (requires fun h0 ->
+    let s1 = Spec.size_of_tree (v_linked_tree l h0) in
+    let s2 = Spec.size_of_tree (v_linked_tree r h0) in
+    s1 + s2 < c - 1)
+  (ensures fun h0 ptr h1 ->
+    let s1 = Spec.size_of_tree (v_linked_tree l h0) in
+    let s2 = Spec.size_of_tree (v_linked_tree r h0) in
+    let s = s1 + s2 + 1 in
+    s < c /\
+    v_linked_tree ptr h1 ==
+    Trees.Node v
+      (v_linked_tree l h0)
+      (v_linked_tree r h0)
+      s)
+  =
+  let s1 = sot_wds l in
+  let s2 = sot_wds r in
+  let s = U.add (U.add s1 s2) one in
+  let sr = malloc s in
+  let n = mk_node v l r sr in
+  let ptr = malloc n in
+  pack_tree ptr l r sr;
+  return ptr
 
 let rec append_left #a (ptr: t a) (v: a)
   : Steel (t a)
@@ -222,47 +311,6 @@ let rec member (#a: eqtype) (ptr: t a) (v: a)
       (**) pack_tree ptr (get_left node) (get_right node) (get_size node);
       return (mleft || mright)
     )
-  )
-
-let sot_wds (#a: Type) (ptr: t a)
-  : Steel (U.t)
-  (linked_tree ptr)
-  (fun _ -> linked_tree ptr)
-  (requires fun _ -> True)
-  (ensures (fun h0 s h1 ->
-    v_linked_tree ptr h0 == v_linked_tree ptr h1 /\
-    U.v s == Spec.sot_wds (v_linked_tree ptr h0) /\
-    U.v s == Spec.size_of_tree (v_linked_tree ptr h0)
-  ))
-  =
-  if is_null_t ptr then (
-    assert (is_null_t ptr);
-    elim_linked_tree_leaf ptr;
-    let h = get () in
-    assert (0 == Spec.sot_wds (v_linked_tree ptr h));
-    return zero
-  ) else (
-    let h1 = get () in
-    (**) let node = unpack_tree ptr in
-    let h2 = get () in
-    let ptr_t1 = hide (v_linked_tree ptr h1) in
-    let ptr_t2 = hide (Spec.Node
-      (get_data (sel ptr h2))
-      (v_linked_tree (get_left node) h2)
-      (v_linked_tree (get_right node) h2)
-      (U.v (sel (get_size node) h2))
-    ) in
-    assert (reveal ptr_t1 == reveal ptr_t2);
-    assert (fst (Spec.is_wds (reveal ptr_t1)));
-    let ptr_s1 = hide (Spec.csize ptr_t1) in
-    let ptr_s2 = hide (Spec.csize ptr_t2) in
-    assert (reveal ptr_s1 == reveal ptr_s2);
-    Spec.check (reveal ptr_t1);
-    assert (reveal ptr_s1 == Spec.size_of_tree (reveal ptr_t1));
-    let s = read (get_size node) in
-    assert (U.v s == Spec.sot_wds (v_linked_tree ptr h1));
-    pack_tree ptr (get_left node) (get_right node) (get_size node);
-    return s
   )
 
 
