P1_UInt32.fst
@@ -32,14 +32,16 @@ let mk_node = NTreeC3.mk_node #U32.t
 
 (* not inlined *)
 let unpack_tree = NTreeC3.unpack_tree #U32.t
-let create_leaf = NTreeC3.create_leaf #U32.t
 
 (* stdlib *)
+let create_leaf = P1.create_leaf #U32.t
+let create_tree = P1.create_tree #U32.t
+let merge_tree = P1.merge_tree #U32.t
+let sot_wds = P1.sot_wds #U32.t
 let append_left = P1.append_left #U32.t
 let append_right = P1.append_right #U32.t
 let height = P1.height #U32.t
 let member = P1.member #U32.t
-let sot_wds = P1.sot_wds #U32.t
 let rotate_left = P1.rotate_left #U32.t
 let rotate_right = P1.rotate_right #U32.t
 let rotate_right_left = P1.rotate_right_left #U32.t
@@ -94,13 +96,7 @@ let main ()
   (requires fun _ -> True)
   (ensures fun _ _ _-> True)
   =
-  let l = create_leaf () in
-  let r = create_leaf () in
-  let sr = malloc 1UL in
-  let v = 1ul in
-  let n = mk_node v l r sr in
-  let ptr = malloc n in
-  NTreeC3.pack_tree ptr l r sr;
+  let ptr = create_tree 1ul in
   let ptr = append_left ptr 0ul in
   let b = member ptr 0ul in
   let vr = if b then 42ul else 11ul in
